Introduce impl/spec_couplable and refactor hash coupling lemma

theories/examples/hash.v
@@ -868,6 +868,98 @@ Section tape_bit_hash.
       }
   Qed.
 
+  Definition impl_couplable (P : bool → iProp Σ) : iProp Σ :=
+    (∃ α bs, α ↪ bs ∗ (∀ b, α ↪ (bs ++ [b]) -∗ P b)).
+  Definition spec_couplable (P : bool → iProp Σ) : iProp Σ :=
+    (∃ α bs, α ↪ₛ bs ∗ (∀ b, α ↪ₛ (bs ++ [b]) -∗ P b)).
+
+  Lemma hashfun_couplable k max f m :
+    k ≤ max →
+    m !! k = None →
+    hashfun max f m -∗ impl_couplable (λ b, hashfun max f (<[k:=b]>m)).
+  Proof.
+    iIntros (Hmax Hlookup) "Hhashfun".
+    iDestruct "Hhashfun" as (lvm ltm vm tm Hdom1 Hdom2 ->) "(Hvm&Htm&Htapes)".
+    (* Get the tape id for k *)
+    assert (is_Some (tm !! k)) as (α&Hα).
+    { apply elem_of_dom. apply Hdom1. lia. }
+
+    iDestruct (big_sepM_delete with "Htapes") as "(Hk&Htapes)"; first eauto.
+    iDestruct "Hk" as "[Hbad|[Hbad|Hk]]".
+    { iExFalso. iDestruct "Hbad" as (?) "(%Hbadlook&_)". congruence. }
+    { iExFalso. iDestruct "Hbad" as (?) "(%Hbadlook&_)". congruence. }
+    iDestruct "Hk" as "(%Hnone1&%Hnone2&Hα)".
+
+    rewrite /impl_couplable. iExists α, [].
+    iFrame. iIntros (b) "Hα".
+    iExists _, _, _, _. iFrame.
+    iSplit; first done.
+    iSplit.
+    { iPureIntro; split; intuition auto. rewrite dom_insert_L.
+      set_solver. }
+    iSplit; first done.
+    iApply big_sepM_delete; first eauto.
+    iSplitL "Hα".
+    { iRight. iLeft. iExists b. iFrame. iPureIntro; split; auto. rewrite lookup_insert //. }
+    iApply (big_sepM_mono with "Htapes").
+    iIntros (k' x' Hdel) "H".
+    assert (k ≠ k').
+    { apply lookup_delete_Some in Hdel. intuition auto. }
+    rewrite ?lookup_insert_ne //.
+  Qed.
+
+  Lemma shashfun_couplable k max f m :
+    k ≤ max →
+    m !! k = None →
+    shashfun max f m -∗ spec_couplable (λ b, shashfun max f (<[k:=b]>m)).
+  Proof.
+    iIntros (Hmax Hlookup) "Hhashfun".
+    iDestruct "Hhashfun" as (lvm ltm vm tm Hdom1 Hdom2 ->) "(Hvm&Htm&Htapes)".
+    (* Get the tape id for k *)
+    assert (is_Some (tm !! k)) as (α&Hα).
+    { apply elem_of_dom. apply Hdom1. lia. }
+
+    iDestruct (big_sepM_delete with "Htapes") as "(Hk&Htapes)"; first eauto.
+    iDestruct "Hk" as "[Hbad|[Hbad|Hk]]".
+    { iExFalso. iDestruct "Hbad" as (?) "(%Hbadlook&_)". congruence. }
+    { iExFalso. iDestruct "Hbad" as (?) "(%Hbadlook&_)". congruence. }
+    iDestruct "Hk" as "(%Hnone1&%Hnone2&Hα)".
+
+    rewrite /spec_couplable. iExists α, [].
+    iFrame. iIntros (b) "Hα".
+    iExists _, _, _, _. iFrame.
+    iSplit; first done.
+    iSplit.
+    { iPureIntro; split; intuition auto. rewrite dom_insert_L.
+      set_solver. }
+    iSplit; first done.
+    iApply big_sepM_delete; first eauto.
+    iSplitL "Hα".
+    { iRight. iLeft. iExists b. iFrame. iPureIntro; split; auto. rewrite lookup_insert //. }
+    iApply (big_sepM_mono with "Htapes").
+    iIntros (k' x' Hdel) "H".
+    assert (k ≠ k').
+    { apply lookup_delete_Some in Hdel. intuition auto. }
+    rewrite ?lookup_insert_ne //.
+  Qed.
+
+  Lemma couplable_elim E e P Q Φ :
+    to_val e = None →
+    nclose specN ⊆ E →
+    spec_ctx ∗ spec_couplable P ∗ impl_couplable Q ∗
+    ((∃ b, P b ∗ Q b) -∗ WP e @ E {{ Φ }})
+    ⊢ WP e @ E {{ Φ }}.
+  Proof.
+    iIntros (??) "(Hspec_ctx&Hscoupl&Hicoupl&Hwp)".
+    iDestruct "Hscoupl" as (sα sbs) "(Hsα&Hsαclo)".
+    iDestruct "Hicoupl" as (α bs) "(Hα&Hαclo)".
+    iApply (wp_couple_tapes with "[-]"); try done; iFrame "Hsα Hα Hspec_ctx".
+    iDestruct 1 as (b) "(Hsα&Hα)". iApply "Hwp".
+    iExists b. iSplitL "Hsα Hsαclo".
+    { iApply "Hsαclo". iFrame. }
+    { iApply "Hαclo". iFrame. }
+  Qed.
+
   Lemma wp_couple_hash E e f sf max m sm k sk Φ :
     (* Both keys need to be in hash domain *)
     k ≤ max →
@@ -882,67 +974,11 @@ Section tape_bit_hash.
     ⊢ WP e @ E {{ Φ }}.
   Proof.
     iIntros (Hmax Hsmax Hlookup Hslookup Hval Hspec) "(Hspec_ctx&Hhashfun&Hshashfun&Hwp)".
-    iDestruct "Hhashfun" as (lvm ltm vm tm Hdom1 Hdom2 ->) "(Hvm&Htm&Htapes)".
-    iDestruct "Hshashfun" as (lsvm lstm svm stm Hsdom1 Hsdom2 ->) "(Hsvm&Hstm&Hstapes)".
-
-    (* Get the tape ids for k and sk *)
-    assert (is_Some (tm !! k)) as (α&Hα).
-    { apply elem_of_dom. apply Hdom1. lia. }
-
-    assert (is_Some (stm !! sk)) as (sα&Hsα).
-    { apply elem_of_dom. apply Hsdom1. lia. }
-    
-    iDestruct (big_sepM_delete with "Htapes") as "(Hk&Htapes)"; first eauto.
-    iDestruct "Hk" as "[Hbad|[Hbad|Hk]]".
-    { iExFalso. iDestruct "Hbad" as (?) "(%Hbadlook&_)". congruence. }
-    { iExFalso. iDestruct "Hbad" as (?) "(%Hbadlook&_)". congruence. }
-    iDestruct "Hk" as "(%Hnone1&%Hnone2&Hα)".
-
-    iDestruct (big_sepM_delete with "Hstapes") as "(Hsk&Hstapes)"; first eauto.
-    iDestruct "Hsk" as "[Hbad|[Hbad|Hsk]]".
-    { iExFalso. iDestruct "Hbad" as (?) "(%Hbadlook&_)". congruence. }
-    { iExFalso. iDestruct "Hbad" as (?) "(%Hbadlook&_)". congruence. }
-    iDestruct "Hsk" as "(%Hsnone1&%Hsnone2&Hsα)".
-
-    (* Couple the tapes *)
-    iApply (wp_couple_tapes with "[-]"); [ auto | auto |].
-    iFrame "Hspec_ctx Hα Hsα". iDestruct 1 as (b) "(Hsα&Hα)".
-
-    iApply "Hwp".
-    iExists b.
-    iSplitL "Hvm Htm Htapes Hα".
-    {
-      iExists _, _, _, _. iFrame.
-      iSplit; first done.
-      iSplit.
-      { iPureIntro; split; intuition auto. rewrite dom_insert_L.
-        set_solver. }
-      iSplit; first done.
-      iApply big_sepM_delete; first eauto.
-      iSplitL "Hα".
-      { iRight. iLeft. iExists b. iFrame. iPureIntro; split; auto. rewrite lookup_insert //. }
-      iApply (big_sepM_mono with "Htapes").
-      iIntros (k' x' Hdel) "H".
-      assert (k ≠ k').
-      { apply lookup_delete_Some in Hdel. intuition auto. }
-      rewrite ?lookup_insert_ne //. 
-    }
-    {
-      iExists _, _, _, _. iFrame.
-      iSplit; first done.
-      iSplit.
-      { iPureIntro; split; intuition auto. rewrite dom_insert_L.
-        set_solver. }
-      iSplit; first done.
-      iApply big_sepM_delete; first eauto.
-      iSplitL "Hsα".
-      { iRight. iLeft. iExists b. iFrame. iPureIntro; split; auto. rewrite lookup_insert //. }
-      iApply (big_sepM_mono with "Hstapes").
-      iIntros (k' x' Hdel) "H".
-      assert (sk ≠ k').
-      { apply lookup_delete_Some in Hdel. intuition auto. }
-      rewrite ?lookup_insert_ne //. 
-    }
+    iDestruct (hashfun_couplable k with "Hhashfun") as "Hhashfun"; try eauto.
+    iDestruct (shashfun_couplable sk with "Hshashfun") as "Hshashfun"; try eauto.
+    iApply (couplable_elim); try done.
+    iFrame "Hspec_ctx Hshashfun Hhashfun".
+    iIntros "H". iApply "Hwp". iDestruct "H" as (b) "(?&?)". iExists _; by iFrame.
   Qed.
 
 End tape_bit_hash.
